### 14.6.3 The Binominal Theorem

`\begin{eqnarray*}
(a+b)^4 &=& aaaa+bbbb+aaba+aabb \\
        & & +abaa+abab+abba+abbb \\
        & & +baaa+baab+baba+babb \\
        & & +bbaa+bbab+bbba+bbbb
\end{eqnarray*}`

`\[
\frac{n!}{k!(n-k)!}=\left(
\begin{array}{c}
  n \\
  k
\end{array}
\right)
\]`

`$ a^{n-k}b^k\mbox{is}\left(\begin{array}{c}  n \\  k \end{array}\right) $`

`\[
(a+b)^4=\left(\begin{array}{c}  4 \\  0 \end{array}\right)\cdot a^4b^0+\left(\begin{array}{c}  4 \\  1 \end{array}\right) \cdot a^3b^1+\left(\begin{array}{c}  4 \\  2 \end{array}\right)\cdot a^2b^2\left(\begin{array}{c}  4 \\  3 \end{array}\right)\cdot a^1b^3+\left(\begin{array}{c}  4 \\  4 \end{array}\right)\cdot a^0b^4
\]`

`\[
(a+b)^n=\sum_{k=0}^{n}\left(\begin{array}{c}  n \\  k \end{array}\right)a^{n-k}b^k
\]`

`\[
bo^2k^2e^3pr
\]`

`\[
\left(\begin{array}{c}  10 \\  1,2,2,3,1,1 \end{array}\right)=\frac{10!}{1!2!2!3!1!1!}
\]`

`\[
(z_1+z_2+\cdots +z_m)^n=\sum_{\begin{array}{c} k_1,\cdots,k_m\in N \\ k_1+\cdots +k_m=n\end{array}}\left(\begin{array}{c}n \\ k_1,k_2,\cdots ,k_m\end{array}\right)Z_1^{k_1}Z_2^{k_2}\cdots Z_m^{k_m}
\]`
